imp/example/IPMAux.v
@@ -1,0 +1,20 @@
+Require Import Coqlib.
+Require Export sflib.
+Require Export AList.
+Require Import Skeleton.
+Require Import Algebra.
+Require Import ModSem Mod ModSemFacts ModFacts.
+Require Import HTactics.
+
+Require Import IPM.
+
+Set Implicit Arguments.
+
+Section AUX.
+
+  Context `{Sk.ld}.
+
+  Definition OwnM (m: Mod.t) : (@mProp (MRA_to_MRAS (Mod_MRA))) :=
+    Own ((m: Mod_MRA.(MRA.car)) : (MRA_to_MRAS Mod_MRA).(MRAS.car)).
+
+End AUX.
